\chapter{Correctness Proofs}
In this chapter we will show two different methods that can be used to prove the correctness of a \textsl{Python}
function.
\begin{enumerate}[(a)]
\item The method of \blue{computational induction} can be used to verify the correctness of a \textsl{Python}
      function that is defined recursively.
\item In order to establish the correctness of a \textsl{Python} function that is defined iteratively we use
      \blue{symbolic execution}. 
\end{enumerate}

\section{Computational Induction}
Figure \ref{fig:power.py} shows the definition of the function $\mytt{power}(m,n)$ that computes
the value $m^n$.  We will verify the correctness of this function.

\begin{figure}[!h]
  \centering
\begin{minted}[ frame         = lines, 
                framesep      = 0.3cm, 
                numbers       = left,
                numbersep     = -0.2cm,
                bgcolor       = sepia,
                xleftmargin   = 0.8cm,
                xrightmargin  = 0.8cm
              ]{python3}
    def power(m, n):
        if n == 0:
            return 1
        p = power(m, n // 2)
        if n % 2 == 0:
            return p * p
        else:
            return p * p * m
\end{minted}
\vspace*{-0.3cm}
  \caption{Computation of $m^n$ for $m,n \in \mathbb{N}$.}
  \label{fig:power.py}
\end{figure} 

It is by no means obvious that the program shown in \ref{fig:power.py} does compute
$m^n$.  We prove this claim by  \blue{computational induction}\index{computational induction}.
Computational induction is an induction on the number of recursive invocations.
This method is the method of choice to prove the correctness of a function if this function is defined recursively.
A proof by computational induction consists of three parts:
\pagebreak

\begin{enumerate}
\item The \blue{base case}.

      In the base case we have to show that the function definition is correct in all those cases where the function
      does not invoke itself recursively.
\item The \blue{induction step}.

      In the induction step we have to prove that the function definition works in all those cases where
      the function does invoke itself recursively.  In order to carry out this proof we may
      assume that the results computed by the recursively invocations are correct.
      This assumption is called the \blue{induction hypotheses}.
\item The \blue{termination proof}.

      In this final step we have to show that the recursive definition of the function is \blue{well founded},
      i.e.~we have to prove that the recursive invocations terminate.
\end{enumerate}
Let us prove the claim 
\\[0.2cm]
\hspace*{1.3cm}
 $\mytt{power}(m,n) = m^n$
\\[0.2cm] 
by computational induction.
\begin{enumerate}
\item \textbf{Base case}:

      The only case where \mytt{power} does not invoke itself recursively is the case $n = 0$.  
      In this case, we have
      \\[0.2cm]
      \hspace*{1.3cm} 
      $\mytt{power}(m,0) = 1 =  m^0$. \mycheck
\item \textbf{Induction step}:

      The recursive invocation of $\mytt{power}$ has the form
      $\mytt{power}(m,n \dv 2)$.  By the induction hypotheses we may assume that 
      \\[0.2cm]
      \hspace*{1.3cm}
      $\displaystyle \mytt{power}(m,n \dv 2) = m^{n \dvv 2}$ 
      \\[0.2cm]
      holds.  After the recursive invocation there are two cases that have to be dealt with separately.
      \begin{enumerate}
      \item $n \;\mytt{\%}\; 2 = 0$, therefore $n$ is even.

            Then there exists a number $k \in \mathbb{N}$ such that $n = 2 \cdot k$ and therefore
            $n \dv 2 = k$.
            Hence we have:
            \\[0.2cm]
            \hspace*{1.3cm}
           $ 
            \begin{array}{lcl}
            \mytt{power}(m,n) & = & \mytt{power}(m,k) \cdot \mytt{power}(m,k) \\[0.2cm]
                                & \stackrel{\mathrm{IV}}{=} & m^k \cdot m^k  \\[0.2cm]
                                & = & m^{2\cdot k} \\[0.2cm]
                                & = & m^{n}.
            \end{array}
            $            
      \item $n \;\mytt{\%}\; 2 = 1$, therefore $n$ is odd.

            Then there exists a number $k \in \mathbb{N}$ such that $n = 2 \cdot k + 1$ and we have
            $n \dv 2 = k$.  In this case we have:
            \\[0.2cm]
            \hspace*{1.3cm}
            $ 
            \begin{array}{lcl}
            \mytt{power}(m,n) & = & \mytt{power}(m,k) \cdot \mytt{power}(m,k) \cdot m  \\[0.2cm]
                                & \stackrel{\mathrm{IV}}{=} & m^k \cdot m^k \cdot m  \\[0.2cm]
                                & = & m^{2\cdot k+1} \\[0.2cm]
                                & = & m^{n}.
            \end{array}
            $
      \end{enumerate}
      As we have shown that $\mytt{power}(m,n) = m^n$ in both cases, the induction step is finished. \mycheck
\item \textbf{Termination proof}:
      Every time the function \mytt{power} is invoked as $\mytt{power}(m, n)$ and $n > 0$, the recursive
      invocation has the form $\mytt{power}(m,n \dv 2)$ and, since $n \dv 2 < n$ for all $n > 0$, the second
      argument is decreased.  As this argument is a natural number, it must eventually reach $0$.  But if the
      second argument of the function $\mytt{power}$ is $0$, the function terminates immediately. \mycheck
      \qed
\end{enumerate}

\begin{figure}[!h]
  \centering
\begin{minted}[ frame         = lines, 
                framesep      = 0.3cm, 
                numbers       = left,
                numbersep     = -0.2cm,
                bgcolor       = sepia,
                xleftmargin   = 0.8cm,
                xrightmargin  = 0.8cm
                ]{python3}
    def div_mod(m, n):
        if m < n:
            return 0, m
        q, r = div_mod(m // 2, n)
        if 2 * r + m % 2 < n:
            return 2 * q, 2 * r + m % 2
        else:
            return 2 * q + 1, 2 * r + m % 2 - n                
\end{minted}
\vspace*{-0.3cm}
  \caption{The function \mytt{div\_mod}.}
  \label{fig:div_mod}
\end{figure} 


\exampleEng
The function \mytt{div\_mod} that is shown in Figure \ref{fig:div_mod} satisfies the specification
\\[0.2cm]
\hspace*{1.3cm}
$\mytt{div\_mod}(m, n) = (q, r)  \rightarrow m = q \cdot n + r \;\wedge\; r < n$. \eox



\proof
Assume that $m,n \in \mathbb{N}$, where $n > 0$.  Furthermore, assume
\\[0.2cm]
\hspace*{1.3cm}
$\bar{q}, \bar{r} = \mytt{div\_mod}(m, n)$.
\\[0.2cm] 
In order to prove the correctness of \mytt{div\_mod}, we have to show two formulas:
\begin{align}
m = \bar{q} \cdot n + \bar{r} \label{divmod1} \\
\bar{r} < n \label{divmod2}
\end{align}
Since \mytt{div\_mod} is defined recursively, the proof of these formulas is done by computational induction.
\begin{enumerate}
\item[B.C.:] $m < n$

  In this case we have $\bar{q} = 0$ and $\bar{r} = m$.
  In order to prove (\ref{divmod1}) we note that 
  \begin{align*}
                    & m = \bar{q} \cdot n + \bar{r} \\
    \Leftrightarrow\quad & m = 0 \cdot n + m \quad \green{\surd}
  \end{align*}
  To prove (\ref{divmod2}) we note that
  \begin{align*}
                         & \bar{r} < n \\
    \Leftrightarrow\quad & m < n \quad\green{\surd}
  \end{align*}
  Here $m < n$ is true because this condition is the assumption of the base case.
\item[I.S.:] $m \dv 2 \mapsto m$

  By induction hypotheses we know that our claim is true for the recursive invocation of \mytt{div\_mod} in
  line 4.  Therefore we have the following:
  \begin{eqnarray}
    m \dv 2 &\!=\! & q \cdot n + r \label{divmod3} \\
          r &\!<\! & n             \label{divmod4}
  \end{eqnarray}
  In order to complete the induction step we have to perform a case distinction that is analogous to the test
  of the second \texttt{if}-statement in the implementation of \mytt{div\_mod}.
  \begin{enumerate}
  \item $2 \cdot r + m \mmod 2 < n$

    In this case we have $\bar{q} = 2 \cdot q$ and $\bar{r} = 2 \cdot r + m \mmod 2$.
    In order to prove (\ref{divmod1}) we note the following:
    \begin{align}
                           &  m = \bar{q} \cdot n + \bar{r} \\
      \Leftrightarrow\quad & m = 2 \cdot q \cdot n + 2 \cdot r + m \mmod 2 \label{divmod5}
    \end{align}
    We will derive equation (\ref{divmod5}) from equation (\ref{divmod3}).  To this end, we multiply equation
    (\ref{divmod3}) by $2$.  This yields:
    \\[0.2cm]
    \hspace*{1.3cm}
    $2 \cdot m \dv 2 = 2 \cdot q \cdot n + 2 \cdot r$.
    \\[0.2cm]
    If we add $m \mmod 2$ to this equation we get
    \\[0.2cm]
    \hspace*{1.3cm}
    $2 \cdot m \dv 2 + m \mmod 2 = 2 \cdot q \cdot n + 2 \cdot r + m \mmod 2$.
    \\[0.2cm]
    As we have $2 \cdot m \dv 2 + m \mmod 2 = m$ the last equation can be simplified to
    \\[0.2cm]
    \hspace*{1.3cm}
    $m = 2 \cdot q \cdot n + 2 \cdot r + m \mmod 2$.
    \\[0.2cm]
    However, this is just equation (\ref{divmod5}) which we had to prove. \mycheck

    Next, we show that $\bar{r} < n$.  This is equivalent to
    \\[0.2cm]
    \hspace*{1.3cm}
    $2 \cdot r + m \mmod 2 < n$.
    \\[0.2cm]
    However, this inequation is the condition of this case of the case distinction and is therefore valid. \mycheck
  \item $2 \cdot r + m \mmod 2 \geq n$

    In this case we have $\bar{q} = 2 \cdot q + 1$ and $\bar{r} = 2 \cdot r + m \mmod 2 - n$.
    We start with the proof of (\ref{divmod1}).
    \begin{align*}
                           & m = \bar{q} \cdot n + \bar{r} \\
      \Leftrightarrow\quad & m = (2 \cdot q + 1) \cdot n + 2 \cdot r + m \mmod 2 - n \\
      \Leftrightarrow\quad & m = 2 \cdot q \cdot n + 2 \cdot r + m \mmod 2 
    \end{align*}
    This last equation follows from equation (\ref{divmod3}) as follows:
    \begin{align*}
                       & m \dv 2 = q \cdot n + r \\
      \Rightarrow\quad & 2 \cdot m \dv 2 = 2 \cdot q \cdot n + 2 \cdot r \\
      \Rightarrow\quad & 2 \cdot m \dv 2 + m \mmod 2 = 2 \cdot q \cdot n + 2 \cdot r + m \mmod 2 \\
      \Rightarrow\quad & m = 2 \cdot q \cdot n + 2 \cdot r + m \mmod 2 
    \end{align*}

    Next, we show that $\bar{r} < n$. This is equivalent to
    \\[0.2cm]
    \hspace*{1.3cm}
    $2 \cdot r + m \mmod 2 - n < n$
    \\[0.2cm]
    From (\ref{divmod4}) we know that
    \begin{align*}
                       & r < n \\
      \Rightarrow\quad & r + 1 \leq n \\
      \Rightarrow\quad & 2 \cdot r + 2 \leq 2 \cdot n \\
      \Rightarrow\quad & 2 \cdot r + m \mmod 2 + 1 \leq 2 \cdot n \quad \mbox{since $m \mmod 2 \leq 1$} \\
      \Rightarrow\quad & 2 \cdot r + m \mmod 2 < 2 \cdot n \\
      \Rightarrow\quad & 2 \cdot r + m \mmod 2 - n < n \green{\surd}
    \end{align*}
  \end{enumerate}
\item[T.:] As $m \dv 2 < m$ for all $m \geq n$ and $n > 0$ it is obvious that we will eventually have
  $m  < n$. But then the function \mytt{div\_mod} terminates.
\end{enumerate}

\begin{figure}[!h]
  \centering
\begin{minted}[ frame         = lines, 
                framesep      = 0.3cm, 
                numbers       = left,
                numbersep     = -0.2cm,
                bgcolor       = sepia,
                xleftmargin   = 0.8cm,
                xrightmargin  = 0.8cm
                ]{python3}
    def gcd(x, y):
        if y == 0:
            return x
        return gcd(y, x % y)
\end{minted}
\vspace*{-0.3cm}
  \caption{The function \mytt{gcd}.}
  \label{fig:gcd}
\end{figure}

\exercise
Prove that the function \mytt{gcd} that is shown in Figure \ref{fig:gcd} computes the greatest common divisor
of its arguments. \eox

\begin{figure}[!h]
  \centering
\begin{minted}[ frame         = lines, 
                framesep      = 0.3cm, 
                numbers       = left,
                numbersep     = -0.2cm,
                bgcolor       = sepia,
                xleftmargin   = 0.8cm,
                xrightmargin  = 0.8cm
                ]{python3}
    def isqrt(n):
        if n == 0:
            return 0
        r = isqrt(n // 4)
        if (2 * r + 1) ** 2 <= n:
            return 2 * r + 1
        else:
            return 2 * r
\end{minted}
\vspace*{-0.3cm}
  \caption{The function \mytt{isqrt}.}
  \label{fig:isqrt}
\end{figure} 




\exerciseEng
The \blue{integer square root} of a natural number $n$ is defined as 
\\[0.2cm]
\hspace*{1.3cm}
$\texttt{isqrt}(n) := \max\bigl(\{ r \in \mathbb{N} \mid r^2 \leq n \}\bigr)$.
\\[0.2cm]
Prove that the function \mytt{isqrt} that is shown in Figure \ref{fig:isqrt} on page \pageref{fig:isqrt}
computes the integer square root of its argument. \eox





\section{Symbolic Execution}
In the last chapter we have seen how to prove the correctness of a recursive function via
\blue{computational induction}.  If a function is implemented via loops instead of recursion, then the method
of computational induction is not applicable.  Therefore, this section introduces the method of
\blue{symbolic execution}. \index{symbolic execution}  Using this method it is possible to verify the
correctness of programs that are implemented in an iterative fashion using loops. 
We will introduce this method via a simple example.  Consider the program shown in Figure
\ref{fig:power-iterative-annotated.stlx}. 

\begin{figure}[!h]
\centering
\begin{Verbatim}[ frame         = lines, 
                  framesep      = 0.3cm, 
                  labelposition = bottomline,
                  numbers       = left,
                  numbersep     = -0.2cm,
                  xleftmargin   = 1.3cm,
                  xrightmargin  = 1.3cm,
                  codes         = {\catcode`_=8\catcode`$=3},
                  commandchars  = \\\{\},
                ]
    \colorbox{sepia}{\green{def} \blue{power}(x$_1$, y$_1$):}
    \colorbox{sepia}{    r$_1$ = 1}
    \colorbox{sepia}{    \green{while} y$_n$ > 0:}
    \colorbox{sepia}{        \green{if} y$_n$ % 2 == 1:}
    \colorbox{sepia}{            r$_{n+1}$ = r$_n$ * x$_n$}
    \colorbox{sepia}{        x$_{n+1}$ = x$_n$ * x$_n$}
    \colorbox{sepia}{        y$_{n+1}$ = y$_n$ // 2}
    \colorbox{sepia}{    \green{return} r$_N$}
\end{Verbatim}
\vspace*{-0.3cm}
\caption{An annotated programm to compute powers.}
\label{fig:power-iterative-annotated.stlx}
\end{figure} % $

The main difference between a mathematical formula and a program is that in a formula all
occurrences of a variable refer to the same value.   This is different in a program because the
variables change their values dynamically.  In order to deal with this property of program variables,
we have to be able to distinguish the different occurrences of a given variable.  To this end,  we 
\blue{index} the program variables. 
When doing this, we have to be aware of the fact that the same occurrence of a program variable can
still denote different values if the variable occurs inside  a loop.  In this case we have to index
the variables in a way such that the index includes a counter that counts the number of loop iterations.
For concreteness, consider the  program shown in 
Figure \ref{fig:power-iterative-annotated.stlx}.  
Here, in line 5 the variable \mytt{r} has the index $n$ on the right side of the assignment,
while it has the index $r_{n+1}$ on the left side of the assignment in line 5.  The index $n$ denotes 
the number of times that the test \mytt{y$_n$ > 0} of the \mytt{while} loop has been executed.
After the \texttt{while}-loop finishes, the variable $\mytt{r}$ is indexed as
$\mytt{r}_N$ in line 8, where $N$ denotes the total number of times that the test \mytt{y > 0} has been executed.
We show the correctness of the given program next.  Let us define
\\[0.2cm]
\hspace*{1.3cm}
$ a := x_1, \quad b := y_1$.
\\[0.2cm]
We will show that the \mytt{while} loop satisfies the \blue{invariant}
\begin{equation}
  \label{eq:powerInv}
  \ds r_n \cdot x_n^{y_n} = a^b.
\end{equation}
This claim is proven by induction on the number of loop iterations.
\begin{enumerate}
\item[B.C.:] $n=1$.

            Since we have $r_1 = 1$, $x_1 = a$, and $y_1 = b$ we have 
            \\[0.2cm]
            \hspace*{1.3cm}
            $r_n \cdot x_n^{y_n} = r_1 \cdot x_1^{y_1} = 1 \cdot a^{b} = a^b$.
\item[I.S.:] $n \mapsto n + 1$.

            We proof proceeds by a case distinction with respect to the expression $y_n \mmod 2$:
            \begin{enumerate}
            \item $y_n \mmod 2 = 1$.

                  Then we have $y_{n} = 2 \cdot (y_n\dv 2) + 1$ and
                  $r_{n+1} = r_n \cdot x_n$.  Hence
                  \begin{eqnarray*}
                      &   & r_{n+1} \cdot x_{n+1}^{y_{n+1}} \\[0.2cm] 
                      & = & (r_{n} \cdot x_n) \cdot (x_{n} \cdot x_{n})^{y_{n}\dvv 2} \\[0.2cm] 
                      & = & r_{n} \cdot x_n^{2 \cdot (y_{n}\dvv 2) + 1} \\[0.2cm] 
                      & = & r_{n} \cdot x_n^{y_n} \\
                      & \stackrel{i.h.}{=} & a^{b} 
                  \end{eqnarray*}

            \item $y_n \mmod 2 = 0$.

                  Then we have $y_{n} = 2 \cdot (y_n\dv 2)$ and $r_{n+1} = r_n$.
                  Therefore
                  \begin{eqnarray*}
                      &   & r_{n+1} \cdot x_{n+1}^{y_{n+1}} \\[0.2cm] 
                      & = & r_{n} \cdot (x_{n} \cdot x_{n})^{y_{n}\dvv 2} \\[0.2cm] 
                      & = & r_{n} \cdot x_n^{2 \cdot (y_{n} \dvv 2)} \\[0.2cm] 
                      & = & r_{n} \cdot x_n^{y_n} \\
                      & \stackrel{i.h.}{=} & a^{b} 
                  \end{eqnarray*}
            \end{enumerate}
\end{enumerate}
This shows the validity of equation (\ref{eq:powerInv}).   If the \mytt{while} loop
terminates, we must have $y_N = 0$.  If $n=N$, then equation (\ref{eq:powerInv}) yields:
\\[0.2cm]
\hspace*{1.3cm}
$$
\begin{array}[t]{cl}
                 & r_N \cdot x_N^{y_N} = a^b \\
\Leftrightarrow  & r_N \cdot x_N^{0}  = a^b \\
\Leftrightarrow  & r_N \cdot 1       = a^b \\
\Leftrightarrow  & r_N               = a^b
\end{array}
$$
\\[0.2cm]
This shows $r_N = a^b$.  The \mytt{while} loop terminates because we have
\\[0.2cm]
\hspace*{1.3cm}
$y_{n+1} = y_n \dv 2 < y_n$ \quad as long as \quad $y_n > 0$
\\[0.2cm]
and therefore $y_n$ must eventually become $0$.  Thus we have proven that
$\mytt{power}(a,b) =a^b$ holds. \qed

\exerciseEng
Use the method of symbolic program execution to prove the correctness of the implementation of the
\href{https://en.wikipedia.org/wiki/Euclidean_algorithm}{Euclidean algorithm} that is shown in Figure
\ref{fig:gcd.stlx} on page \pageref{fig:gcd.stlx}.  During the proof 
you should make use of the fact that for all positive natural numbers $x$ and $y$ the function $\mytt{ggt}$
that computes the greatest common divisor of $x$ and $x$ satisfies the equation
\\[0.2cm]
\hspace*{1.3cm}
$\mytt{ggt}(x, y) = \mytt{ggt}(x \,\mytt{\%}\, y, y)$.
\\[0.2cm]
Furthermore, the invariant of the \mytt{while} loop is
\\[0.2cm]
\hspace*{1.3cm}
$\mytt{ggt}(x_n, y_n) = \mytt{ggt}(a, b)$ \quad where $a := x_1$ and $b := y_1$.
\\[0.2cm]
Using this invariant you should be able to prove that $\mytt{gcd}(a, b) = \mytt{ggt}(a, b)$ for all
$a, b \in \mathbb{N}$ such that $a > 0$.  Note that in order to carry out the proof you have to distinguish
between the mathematical function \mytt{ggt} that computes the greatest common divisor and the \textsl{Python}
function \mytt{gcd} that is implemented in Figure \ref{fig:gcd.stlx}.
\eox

\begin{figure}[!ht]
\centering
\begin{Verbatim}[ frame         = lines, 
                  framesep      = 0.3cm, 
                  firstnumber   = 1,
                  labelposition = bottomline,
                  numbers       = left,
                  numbersep     = -0.2cm,
                  xleftmargin   = 0.8cm,
                  xrightmargin  = 0.8cm,
                  codes         = {\catcode`_=8\catcode`$=3},
                  commandchars  = \\\{\},
                ]
\colorbox{sepia}{    \green{def} \blue{gcd}(x, y):                    }
\colorbox{sepia}{        \green{while} y != 0:                 }
\colorbox{sepia}{            x, y = y, x % y           }
\colorbox{sepia}{        \green{return} x                      }
\end{Verbatim}
\vspace*{-0.3cm}
\caption{The Euclidean algorithm.}
\label{fig:gcd.stlx}
\end{figure}

\section{Check Your Understanding}
\begin{enumerate}[(a)]
\item Explain the method of \blue{computational induction}.
\item Use the method of computational induction to prove the correctness of the function \texttt{div\_mod}.
\item Explain the method of \blue{symbolic execution}.
\item Use the method of symbolic execution to prove the correctness of Euklid's algorithm.
\item When would you use computational induction and when would you choose symbolic execution instead?
\end{enumerate}

%%% Local Variables:
%%% mode: latex
%%% TeX-master: "logic"
%%% End:
